Some clean up: add bullets, modernize proofs, etc.

src/Lambda/Bidirectional.v
@@ -58,41 +58,35 @@ Fixpoint infer (G : Ctx) (t : tm) : option type :=
 match t with
 | TVar x => G x
 | TApp t1 t2 =>
-    match infer G t1, infer G t2 with
-    | Some (TArr A B), Some A' =>
-            if type_eq_dec A A' then Some B else None
-    | _, _ => None
-    end
+  match infer G t1, infer G t2 with
+  | Some (TArr A B), Some A' => if type_eq_dec A A' then Some B else None
+  | _, _ => None
+  end
 | TLam x t' => None
 | TTrue => Some TBool
 | TFalse => Some TBool
 | TIf t1 t2 t3 =>
-    match infer G t1, infer G t2, infer G t3 with
-    | Some TBool, Some A, Some A' =>
-            if type_eq_dec A A' then Some A else None
-    | _, _, _ => None
-    end
+  match infer G t1, infer G t2, infer G t3 with
+  | Some TBool, Some A, Some A' => if type_eq_dec A A' then Some A else None
+  | _, _, _ => None
+  end
 end.
 
 Lemma type_eq_dec_refl :
   forall A : type, type_eq_dec A A = true.
 Proof.
-  induction A; cbn.
-    reflexivity.
-    rewrite IHA1, IHA2. cbn. reflexivity.
+  induction A; cbn; [easy |].
+  now rewrite IHA1, IHA2; cbn.
 Qed.
 
 Lemma has_type_infer :
   forall (G : Ctx) (x : tm) (A : type),
     has_type G x A -> infer G x = Some A.
 Proof.
-  induction 1; cbn.
-    assumption.
-    rewrite IHhas_type1, IHhas_type2, type_eq_dec_refl. reflexivity.
-    admit. (* lambda *)
-    1-2: reflexivity.
-    rewrite IHhas_type1, IHhas_type2, IHhas_type3, type_eq_dec_refl.
-      reflexivity.
+  induction 1; cbn; only 1, 4-5: easy.
+  - now rewrite IHhas_type1, IHhas_type2, type_eq_dec_refl.
+  - admit. (* lambda *)
+  - now rewrite IHhas_type1, IHhas_type2, IHhas_type3, type_eq_dec_refl.
 Admitted.
 
 End STLC_with_Booleans.
@@ -166,10 +160,10 @@ Fixpoint infer (G : Ctx) (t : tm) : option type :=
 match t with
 | TVar x => G x
 | TApp t1 t2 =>
-        match infer G t1 with
-        | Some (TArr A B) => if check G t2 A then Some B else None
-        | _ => None
-        end
+  match infer G t1 with
+  | Some (TArr A B) => if check G t2 A then Some B else None
+  | _ => None
+  end
 | TTrue => Some TBool
 | TFalse => Some TBool
 | TAnn t A => if check G t A then Some A else None
@@ -179,22 +173,22 @@ end
 with check (G : Ctx) (t : tm) (A : type) : bool :=
 match t with
 | TLam x t =>
-    match A with
-    | TArr X Y => check (fun v : V => if x =? v then Some X else G v) t Y
-    | _ => false
-    end
+  match A with
+  | TArr X Y => check (fun v : V => if x =? v then Some X else G v) t Y
+  | _ => false
+  end
 | TIf t1 t2 t3 => check G t1 TBool && check G t2 A && check G t3 A
 (* Not very pretty, but it works. *)
 | TVar x =>
-    match G x with
-    | Some B => type_eq_dec A B
-    | _ => false
-    end
+  match G x with
+  | Some B => type_eq_dec A B
+  | _ => false
+  end
 | TApp t1 t2 =>
-    match infer G t1 with
-    | Some (TArr X Y) => check G t2 X && type_eq_dec Y A
-    | _ => false
-    end
+  match infer G t1 with
+  | Some (TArr X Y) => check G t2 X && type_eq_dec Y A
+  | _ => false
+  end
 | TTrue => type_eq_dec TBool A
 | TFalse => type_eq_dec TBool A
 | TAnn t' A' => check G t' A' && type_eq_dec A A'
@@ -203,9 +197,8 @@ end.
 Lemma type_eq_dec_refl :
   forall A : type, type_eq_dec A A = true.
 Proof.
-  induction A; cbn.
-    reflexivity.
-    rewrite IHA1, IHA2. cbn. reflexivity.
+  induction A; cbn; [easy |].
+  now rewrite IHA1, IHA2; cbn.
 Qed.
 
 Ltac inv H := inversion H; subst; clear H.
@@ -214,22 +207,24 @@ Lemma infer_check :
   forall (G : Ctx) (t : tm) (A : type),
     infer G t = Some A -> check G t A = true.
 Proof.
-  destruct t; cbn; intros.
-    rewrite H. apply type_eq_dec_refl.
-    destruct (infer G t1) as [[] |]; inv H.
-      destruct (check G t2 t); inv H1. cbn. apply type_eq_dec_refl.
-    1-4: inv H; auto.
-    destruct (check G t t0); inv H. cbn. apply type_eq_dec_refl.
+  destruct t; cbn; intros; only 3-6: now inversion H.
+  - now rewrite H, type_eq_dec_refl.
+  - destruct (infer G t1) as [[] |]; [easy | | easy].
+    destruct (check G t2 t); cbn; [| easy].
+    injection H as [= ->].
+    now apply type_eq_dec_refl.
+  - destruct (check G t t0); cbn; [| easy].
+    injection H as [= ->].
+    now apply type_eq_dec_refl.
 Qed.
 
 Lemma type_eq_dec_true :
   forall A B : type,
     type_eq_dec A B = true -> A = B.
 Proof.
-  induction A; destruct B; cbn; intros; try congruence.
-  specialize (IHA1 B1). specialize (IHA2 B2).
-  destruct (type_eq_dec A1 B1), (type_eq_dec A2 B2).
-    all: firstorder; congruence.
+  induction A; destruct B; cbn; intros; only 1-3: easy.
+  apply andb_prop in H as [H1 H2].
+  now rewrite (IHA1 B1), (IHA2 B2).
 Qed.
 
 Lemma infer_correct :
@@ -240,38 +235,46 @@ with check_correct :
   forall (G : Ctx) (t : tm) (A : type),
     check G t A = true -> check_type G t A.
 Proof.
-  destruct t; cbn; intros.
-    constructor. assumption.
-    case_eq (infer G t1); intros; rewrite H0 in H.
+  - destruct t; cbn; intros.
+    + now constructor.
+    + case_eq (infer G t1); intros; rewrite H0 in H; [| easy].
       destruct t; inv H.
       case_eq (check G t2 t3); intro; rewrite H in H2; inv H2.
-        eapply infer_App.
-          eapply infer_correct. exact H0.
-          apply check_correct. assumption.
-    1-5: inversion H; subst; repeat constructor.
-    case_eq (check G t t0); intro; rewrite H0 in H; inv H.
-      constructor. apply check_correct. assumption.
-  destruct t; cbn; intros.
-    case_eq (G v); intros; rewrite H0 in H; inv H.
-      apply type_eq_dec_true in H2; subst. do 2 constructor. assumption.
-    case_eq (infer G t1); intros; rewrite H0 in H.
-      destruct t; inv H.
-      case_eq (check G t2 t3); intro; rewrite H in H2; inv H2.
+      apply infer_App with t3.
+      * now apply infer_correct.
+      * now apply check_correct.
+    + easy.
+    + now inversion H; subst; constructor.
+    + now inversion H; subst; constructor.
+    + easy.
+    + case_eq (check G t t0); intros; rewrite H0 in H; inv H.
+      constructor.
+      now apply check_correct.
+  - destruct t; cbn; intros.
+    + case_eq (G v); intros; rewrite H0 in H; inv H.
+      apply type_eq_dec_true in H2; subst.
+      now do 2 constructor.
+    + case_eq (infer G t1); intros; rewrite H0 in H.
+      * destruct t; inv H.
+        case_eq (check G t2 t3); intro; rewrite H in H2; inv H2.
         apply type_eq_dec_true in H3; subst.
-          constructor. eapply infer_App.
-            apply infer_correct. exact H0.
-            apply check_correct. assumption.
-      congruence.
-    1-3: destruct A; inversion H.
-      constructor. apply check_correct. assumption.
-    do 2 constructor.
-    do 2 constructor.
-    constructor; apply check_correct;
-      destruct (check G t1 TBool), (check G t2 A), (check G t3 A);
-        cbn in H; auto.
-    constructor. case_eq (check G t t0); intros; rewrite H0 in H; inv H.
-      apply type_eq_dec_true in H2; subst. constructor.
-        apply check_correct. assumption.
+        constructor.
+        apply infer_App with t3.
+        -- now apply infer_correct.
+        -- now apply check_correct.
+      * now congruence.
+    + destruct A; inversion H.
+      constructor.
+      now apply check_correct.
+    + destruct A; inversion H.
+      now constructor.
+    + destruct A; inversion H.
+      now constructor.
+    + apply andb_prop in H as [[H1 H2]%andb_prop H3].
+      now constructor; apply check_correct.
+    + apply andb_prop in H as [H1 [= ->]%type_eq_dec_true].
+      do 2 constructor.
+      now apply check_correct.
 Qed.
 
 Lemma infer_complete :
@@ -282,15 +285,14 @@ with check_complete :
   forall (G : Ctx) (t : tm) (A : type),
     check_type G t A -> check G t A = true.
 Proof.
-  destruct 1; cbn; intros.
-    assumption.
-    rewrite (infer_complete _ _ _ H), (check_complete _ _ _ H0). reflexivity.
-    1-2: reflexivity.
-    rewrite (check_complete _ _ _ H). reflexivity.
-  destruct 1; cbn; intros.
-    apply check_complete. assumption.
-    rewrite !check_complete; cbn; auto.
-    apply infer_check. apply infer_complete. apply H.
+  - destruct 1; cbn; intros; only 1, 3-4: easy.
+    + apply infer_complete in H as ->.
+      now apply check_complete in H0 as ->.
+    + now apply check_complete in H as ->.
+  - destruct 1; cbn; intros.
+    + now apply check_complete.
+    + now rewrite !check_complete; cbn.
+    + now apply infer_check, infer_complete.
 Qed.
 
 End Bidirectional_STLC_with_Booleans.
@@ -379,35 +381,33 @@ end
 with check (G : Ctx) (t : tmIn) (A : type) : bool :=
 match t with
 | TLam x t =>
-    match A with
-    | TArr X Y =>
-            check (fun v : V => if x =? v then Some X else G v) t Y
-    | _ => false
-    end
+  match A with
+  | TArr X Y => check (fun v : V => if x =? v then Some X else G v) t Y
+  | _ => false
+  end
 | TIf t1 t2 t3 => check G t1 TBool && check G t2 A && check G t3 A
 | TEx t' =>
-    match infer G t' with
-    | Some B => type_eq_dec A B
-    | _ => false
-    end
+  match infer G t' with
+  | Some B => type_eq_dec A B
+  | _ => false
+  end
 end.
 
 Lemma type_eq_dec_refl :
   forall A : type, type_eq_dec A A = true.
 Proof.
-  induction A; cbn.
-    reflexivity.
-    rewrite IHA1, IHA2. cbn. reflexivity.
+  induction A; cbn; [easy |].
+  now rewrite IHA1, IHA2; cbn.
 Qed.
 
 Lemma type_eq_dec_true :
   forall A B : type,
     type_eq_dec A B = true -> A = B.
 Proof.
-  induction A; destruct B; cbn; intros; try congruence.
-  specialize (IHA1 B1). specialize (IHA2 B2).
-  destruct (type_eq_dec A1 B1), (type_eq_dec A2 B2).
-    all: firstorder; congruence.
+  induction A; destruct B; cbn; intros;
+    only 1-3: easy.
+  apply andb_prop in H as [H1 H2].
+  now rewrite (IHA1 B1), (IHA2 B2).
 Qed.
 
 Ltac inv H := inversion H; subst; clear H.
@@ -420,27 +420,27 @@ with check_correct :
   forall (G : Ctx) (t : tmIn) (A : type),
     check G t A = true -> check_type G t A.
 Proof.
-  destruct t; cbn; intros.
-    constructor. assumption.
-    case_eq (infer G t); intros; rewrite H0 in H.
-      destruct t1; inv H.
-      case_eq (check G t0 t1_1); intro; rewrite H in H2; inv H2.
-      eapply infer_App.
-        eapply infer_correct. exact H0.
-        apply check_correct. assumption.
-      inv H.
-    inv H. constructor.
-    inv H. constructor.
-    case_eq (check G t t0); intro; rewrite H0 in H; inv H.
+  - destruct t; cbn; intros.
+    + constructor. assumption.
+    + case_eq (infer G t); intros; rewrite H0 in H.
+      * destruct t1; inv H.
+        case_eq (check G t0 t1_1); intro; rewrite H in H2; inv H2.
+        eapply infer_App.
+        -- eapply infer_correct. exact H0.
+        -- apply check_correct. assumption.
+      * inv H.
+    + inv H. constructor.
+    + inv H. constructor.
+    + case_eq (check G t t0); intro; rewrite H0 in H; inv H.
       constructor. apply check_correct. assumption.
-  destruct t; cbn; intros.
-    destruct A.
-      inv H.
-      constructor. apply check_correct. assumption.
-    constructor; apply check_correct;
+  - destruct t; cbn; intros.
+    + destruct A.
+      * inv H.
+      * constructor. apply check_correct. assumption.
+    + constructor; apply check_correct;
       destruct (check G t1 TBool), (check G t2 A), (check G t3 A); cbn in H;
       congruence.
-    constructor. apply infer_correct. destruct (infer G t).
+    + constructor. apply infer_correct. destruct (infer G t).
       f_equal. symmetry. apply type_eq_dec_true. assumption.
       inv H.
 Qed.
@@ -453,15 +453,13 @@ with check_complete :
   forall (G : Ctx) (t : tmIn) (A : type),
     check_type G t A -> check G t A = true.
 Proof.
-  destruct 1; cbn; intros.
-    assumption.
-    rewrite (infer_complete _ _ _ H), (check_complete _ _ _ H0). reflexivity.
-    1-2: reflexivity.
-    rewrite (check_complete _ _ _ H). reflexivity.
-  destruct 1; cbn; intros.
-    apply check_complete. assumption.
-    rewrite !check_complete; cbn; auto.
-    rewrite (infer_complete _ _ _ H). apply type_eq_dec_refl.
+  - destruct 1; cbn; intros; only 1, 3-4: easy.
+    + now rewrite (infer_complete _ _ _ H), (check_complete _ _ _ H0).
+    + now rewrite (check_complete _ _ _ H).
+  - destruct 1; cbn; intros.
+    + now apply check_complete.
+    + now rewrite !check_complete; cbn.
+    + now rewrite (infer_complete _ _ _ H), type_eq_dec_refl.
 Qed.
 
 End Bidirectional_STLC_with_Booleans_using_mutual_induction.
@@ -478,12 +476,12 @@ Parameter dec_spec :
 Notation "x =? y" := (dec x y) (at level 70).
 
 Inductive type : Type :=
-| TArr : type -> type -> type
+| TArr   : type -> type -> type
 | TEmpty : type
-| TUnit : type
-| TBool : type
-| TProd : type -> type -> type
-| TSum : type -> type -> type.
+| TUnit  : type
+| TBool  : type
+| TProd  : type -> type -> type
+| TSum   : type -> type -> type.
 
 Inductive tmEx : Type :=
 | TVar : V -> tmEx
@@ -507,12 +505,9 @@ with tmIn : Type :=
 | TEx : tmEx -> tmIn
 | TLam : V -> tmIn -> tmIn
 | TExfalso : tmIn -> tmIn
-(*| TExfalso : tmIn -> type -> tmIn *)
 
 | TInl : tmIn -> tmIn
 | TInr : tmIn -> tmIn.
-
-(*  | TCase *)
 
 Definition Ctx : Type := V -> option type.
 
@@ -557,24 +552,24 @@ Inductive infer_type : Ctx -> tmEx -> type -> Prop :=
 
 with check_type : Ctx -> tmIn -> type -> Prop :=
 | check_Ex :
-        forall (G : Ctx) (t : tmEx) (A : type),
-          infer_type G t A -> check_type G (TEx t) A
+    forall (G : Ctx) (t : tmEx) (A : type),
+      infer_type G t A -> check_type G (TEx t) A
 | check_Lam :
-        forall (G : Ctx) (x : V) (t : tmIn) (A B : type),
-          check_type (fun v : V => if x =? v then Some A else G v) t B ->
-            check_type G (TLam x t) (TArr A B)
+    forall (G : Ctx) (x : V) (t : tmIn) (A B : type),
+      check_type (fun v : V => if x =? v then Some A else G v) t B ->
+        check_type G (TLam x t) (TArr A B)
 (*| check_Exfalso :
-        forall (G : Ctx) (t : tmIn) (A : type),
-          check_type G t TEmpty -> check_type G (TExfalso t A) A *)
+    forall (G : Ctx) (t : tmIn) (A : type),
+      check_type G t TEmpty -> check_type G (TExfalso t A) A *)
 | check_Exfalso :
-        forall (G : Ctx) (t : tmIn) (A : type),
-          check_type G t TEmpty -> check_type G (TExfalso t) A
+    forall (G : Ctx) (t : tmIn) (A : type),
+      check_type G t TEmpty -> check_type G (TExfalso t) A
 | check_Inl :
-        forall (G : Ctx) (t : tmIn) (A B : type),
-          check_type G t A -> check_type G (TInl t) (TSum A B)
+    forall (G : Ctx) (t : tmIn) (A B : type),
+      check_type G t A -> check_type G (TInl t) (TSum A B)
 | check_Inr :
-        forall (G : Ctx) (t : tmIn) (A B : type),
-          check_type G t B -> check_type G (TInr t) (TSum A B).
+    forall (G : Ctx) (t : tmIn) (A B : type),
+      check_type G t B -> check_type G (TInr t) (TSum A B).
 
 #[global] Hint Constructors infer_type : core.
 #[global] Hint Constructors check_type : core.
@@ -593,11 +588,10 @@ end.
 Lemma type_eq_dec_spec :
   forall A B : type, reflect (A = B) (type_eq_dec A B).
 Proof.
-  induction A; destruct B; cbn; try constructor; try inversion 1.
-    destruct (IHA1 B1), (IHA2 B2); cbn; constructor; congruence.
-    1-3: reflexivity.
-    destruct (IHA1 B1), (IHA2 B2); cbn; constructor; congruence.
-    destruct (IHA1 B1), (IHA2 B2); cbn; constructor; congruence.
+  induction A; destruct B; cbn; try (now constructor; try inversion 1).
+  - now destruct (IHA1 B1), (IHA2 B2); cbn; constructor; congruence.
+  - now destruct (IHA1 B1), (IHA2 B2); cbn; constructor; congruence.
+  - now destruct (IHA1 B1), (IHA2 B2); cbn; constructor; congruence.
 Qed.
 
 Fixpoint infer (G : Ctx) (t : tmEx) : option type :=
@@ -605,74 +599,67 @@ match t with
 | TVar x => G x
 | TAnn t A => if check G t A then Some A else None
 | TApp t1 t2 =>
-    match infer G t1 with
-    | Some (TArr A B) => if check G t2 A then Some B else None
-    | _ => None
-    end
+  match infer G t1 with
+  | Some (TArr A B) => if check G t2 A then Some B else None
+  | _ => None
+  end
 | TStar => Some TUnit
 | TTrue => Some TBool
 | TFalse => Some TBool
 | TIf t1 t2 t3 =>
-    match infer G t2, infer G t3 with
-    | Some A, Some B =>
-            if check G t1 TBool && type_eq_dec A B then Some A else None
-    | _, _ => None
-    end
+  match infer G t2, infer G t3 with
+  | Some A, Some B => if check G t1 TBool && type_eq_dec A B then Some A else None
+  | _, _ => None
+  end
 | TPair t1 t2 =>
-    match infer G t1, infer G t2 with
-    | Some A, Some B => Some (TProd A B)
-    | _, _ => None
-    end
+  match infer G t1, infer G t2 with
+  | Some A, Some B => Some (TProd A B)
+  | _, _ => None
+  end
 | TOutl t' =>
-    match infer G t' with
-    | Some (TProd A B) => Some A
-    | _ => None
-    end
+  match infer G t' with
+  | Some (TProd A B) => Some A
+  | _ => None
+  end
 | TOutr t' =>
-    match infer G t' with
-    | Some (TProd A B) => Some B
-    | _ => None
-    end
+  match infer G t' with
+  | Some (TProd A B) => Some B
+  | _ => None
+  end
 | TCase t1 t2 t3 =>
-    match infer G t1, infer G t2, infer G t3 with
-    | Some (TSum A B), Some (TArr A' C), Some (TArr B' C') =>
-        if
-          type_eq_dec A A' &&
-          type_eq_dec B B' &&
-          type_eq_dec C C'
-        then
-          Some C
-        else
-          None
-    | _, _, _ => None
-    end
+  match infer G t1, infer G t2, infer G t3 with
+  | Some (TSum A B), Some (TArr A' C), Some (TArr B' C') =>
+      if type_eq_dec A A' && type_eq_dec B B' && type_eq_dec C C'
+      then Some C
+      else None
+  | _, _, _ => None
+  end
 end
 
 with check (G : Ctx) (t : tmIn) (A : type) : bool :=
 match t with
 | TEx t' =>
-        match infer G t' with
-        | Some B => type_eq_dec A B
-        | _ => false
-        end
+  match infer G t' with
+  | Some B => type_eq_dec A B
+  | _ => false
+  end
 | TLam x t =>
-        match A with
-        | TArr X Y =>
-                check (fun v : V => if x =? v then Some X else G v) t Y
-        | _ => false
-        end
+  match A with
+  | TArr X Y => check (fun v : V => if x =? v then Some X else G v) t Y
+  | _ => false
+  end
 (*| TExfalso t' B => check G t' TEmpty && type_eq_dec A B *)
 | TExfalso t' => check G t' TEmpty
 | TInl t' =>
-        match A with
-        | TSum B C => check G t' B
-        | _ => false
-        end
+  match A with
+  | TSum B C => check G t' B
+  | _ => false
+  end
 | TInr t' =>
-        match A with
-        | TSum B C => check G t' C
-        | _ => false
-        end
+  match A with
+  | TSum B C => check G t' C
+  | _ => false
+  end
 end.
 
 Ltac inv H := inversion H; subst; clear H.
@@ -685,33 +672,38 @@ with check_correct :
   forall (G : Ctx) (t : tmIn) (A : type),
     check G t A = true -> check_type G t A.
 Proof.
-  destruct t; cbn; intros.
-    constructor. assumption.
-    case_eq (check G t t0); intro H'; rewrite H' in H; inv H.
-      constructor. apply check_correct. assumption.
-    case_eq (infer G t).
-      intros C H'. rewrite H' in H. destruct C as []; inv H.
+  - destruct t; cbn; intros.
+    + now constructor.
+    + case_eq (check G t t0); intro H'; rewrite H' in H; inv H.
+      constructor.
+      now apply check_correct.
+    + case_eq (infer G t).
+      * intros C H'.
+        rewrite H' in H.
+        destruct C as []; inv H.
         case_eq (check G t0 C1); intro H''; rewrite H'' in H1; inv H1.
         econstructor.
-          apply infer_correct. exact H'.
-          apply check_correct. assumption.
-      intro H'. rewrite H' in H. inv H.
-    1-3: inv H; constructor.
-    case_eq (infer G t2); [intros t H' | intro H']; rewrite H' in H; inv H.
-      case_eq (infer G t3); [intros t' H'' | intro H''];
-      rewrite H'' in H1; inv H1.
-      case_eq (check G t1 TBool); intro H'''; rewrite H''' in H0; inv H0.
-      destruct (type_eq_dec_spec t t'); subst; inv H1. auto.
-    case_eq (infer G t1); intros; rewrite H0 in *; inv H.
+        -- now eapply infer_correct, H'.
+        -- now apply check_correct.
+      * now intros H'; rewrite H' in H.
+    + now injection H as [= <-]; constructor.
+    + now injection H as [= <-]; constructor.
+    + now injection H as [= <-]; constructor.
+    + case_eq (infer G t2); [intros t H' | intros H']; rewrite H' in H; [| easy].
+      case_eq (infer G t3); [intros t' H'' | intros H'']; rewrite H'' in H; [| easy].
+      case_eq (check G t1 TBool); intro H'''; rewrite H''' in H; [| easy].
+      destruct (type_eq_dec_spec t t'); subst; [| easy].
+      now cbn in H; inversion H; subst; auto.
+    + case_eq (infer G t1); intros; rewrite H0 in *; inv H.
       case_eq (infer G t2); intros; rewrite H in *; inv H2.
       auto.
-    case_eq (infer G t); intros; rewrite H0 in *; inv H.
+    + case_eq (infer G t); intros; rewrite H0 in *; inv H.
       destruct t0; inv H2. econstructor. apply infer_correct.
       cbn. rewrite H0. reflexivity.
-    case_eq (infer G t); intros; rewrite H0 in *; inv H.
+    + case_eq (infer G t); intros; rewrite H0 in *; inv H.
       destruct t0; inv H2. econstructor. apply infer_correct.
       cbn. rewrite H0. reflexivity.
-    case_eq (infer G t1); intros; rewrite H0 in *; try destruct t; inv H.
+    + case_eq (infer G t1); intros; rewrite H0 in *; try destruct t; inv H.
       case_eq (infer G t2); intros; rewrite H in *; try destruct t; inv H2.
       case_eq (infer G t3); intros; rewrite H1 in *; try destruct t; inv H3.
       destruct
@@ -720,19 +712,19 @@ Proof.
         (type_eq_dec_spec t7 t9);
       cbn in *; subst; inv H4; try congruence.
       econstructor; apply infer_correct; eassumption.
-  destruct t; cbn; intros.
-    constructor. apply infer_correct. destruct (infer G t).
+  - destruct t; cbn; intros.
+    + constructor. apply infer_correct. destruct (infer G t).
       f_equal. destruct (type_eq_dec_spec A t0); congruence.
       inv H.
-    destruct A; inv H. constructor. apply check_correct. assumption.
+    + destruct A; inv H. constructor. apply check_correct. assumption.
 (*
     destruct (type_eq_dec_spec A t0); subst.
       constructor. apply check_correct. rewrite andb_true_r in H. assumption.
       rewrite andb_false_r in H. inv H.
 *)
-    constructor. apply check_correct. assumption.
-    destruct A; inv H. constructor. apply check_correct. assumption.
-    destruct A; inv H. constructor. apply check_correct. assumption.
+    + constructor. apply check_correct. assumption.
+    + destruct A; inv H. constructor. apply check_correct. assumption.
+    + destruct A; inv H. constructor. apply check_correct. assumption.
 Qed.
 
 Lemma infer_correct'' :
